More notes in CEK.v

src/CEK.v
@@ -35,21 +35,21 @@ Derive Signature NoConfusion for Value.
 Derive Signature NoConfusion Subterm for Closure.
 Derive Signature NoConfusion for Env.
 
-Inductive represents Γ : ∀ {τ}, Exp Γ τ → Value τ → Prop :=
+Inductive represents {Γ} : ∀ {τ}, Exp Γ τ → Value τ → Prop :=
   | VConst_represents {ty} (l : Literal ty) :
-    represents Γ (Constant l) (VConst l)
-  | VUnit_represents  : represents Γ EUnit VUnit
-  | VTrue_represents  : represents Γ ETrue VTrue
-  | VFalse_represents : represents Γ EFalse VFalse
+    represents (Constant l) (VConst l)
+  | VUnit_represents  : represents EUnit VUnit
+  | VTrue_represents  : represents ETrue VTrue
+  | VFalse_represents : represents EFalse VFalse
   | VPair_represents {τ1 τ2} (x : Exp Γ τ1) x' (y : Exp Γ τ2) y' :
-    represents Γ x x' →
-    represents Γ y y' →
-    represents Γ (Pair x y) (VPair x' y')
+    represents x x' →
+    represents y y' →
+    represents (Pair x y) (VPair x' y')
   | VClosure_represents {dom cod} (e : Exp (dom :: Γ) cod) (ρ : Env Γ) :
-    represents Γ (LAM e) (VClosure (Lambda e ρ)).
+    represents (LAM e) (VClosure (Lambda e ρ)).
 
 Lemma represents_values Γ {τ : Ty} (v : Exp Γ τ) (v' : Value τ) :
-  represents Γ v v' → ValueP v.
+  represents v v' → ValueP v.
 Proof.
   intros.
   now induction H; constructor.
@@ -60,12 +60,14 @@ Equations get `(se : Env Γ) `(v : Var Γ τ) : Value τ :=
   get (Val _ xs) (SV v) := get xs v.
 
 Inductive Kont : Ty → Ty → Type :=
-  | Fn {a b} : (Value a → Σ b + Value b) → Kont a b
+  | Fn {a b} : (Value a → Σ b) → Kont a b
 
 with Σ : Ty → Type :=
-  | MkΣ (τ   : Ty)
-        (Γ   : Exp.Env)
-        (r   : Ty)
+  | MkV {τ   : Ty}
+        (v   : Value τ) : Σ τ
+  | MkΣ {τ   : Ty}
+        {Γ   : Exp.Env}
+        {r   : Ty}
         (exp : Exp Γ r)
         (env : Env Γ)
         (knt : Kont r τ) : Σ τ.
@@ -73,18 +75,15 @@ with Σ : Ty → Type :=
 Derive Signature NoConfusion Subterm for Kont.
 Derive Signature NoConfusion Subterm for Σ.
 
-Arguments MkΣ {τ Γ r} _ _ _.
-
 (* Inject the expression into a [Σ] whose final continuation will receive the
    results of the evaluation. Therefore, the resulting [env] will be a
    singleton list containing that value. *)
-Definition inject {τ : Ty} {Γ : Exp.Env} (e : Exp Γ τ) (E : Env Γ) : Σ τ :=
-  MkΣ e E (Fn inr).
+Definition inject {τ : Ty} (e : Exp [] τ) : Σ τ := MkΣ e Empty (Fn MkV).
 
-Equations IfBody {τ : Ty} {Γ : Exp.Env} (t e : Exp Γ τ)
-          (v : Value TyBool) : Exp Γ τ :=
-  IfBody t _ VTrue  := t;
-  IfBody _ e VFalse := e.
+Equations IfBody (v : Value TyBool) {τ : Ty} {Γ : Exp.Env}
+          (t e : Exp Γ τ) : Exp Γ τ :=
+  IfBody VTrue t _  := t;
+  IfBody VFalse _ e := e.
 
 Equations VFst {τ1 τ2 : Ty} (v : Value (TyPair τ1 τ2)) : Value τ1 :=
   VFst (VPair x _) := x.
@@ -95,37 +94,81 @@ Equations VSnd {τ1 τ2 : Ty} (v : Value (TyPair τ1 τ2)) : Value τ2 :=
 Equations with_closure `(a : Exp Γ dom) (ρ : Env Γ) {τ} `(κ : Kont cod τ)
           `(v : Value (dom ⟶ cod)) : Σ τ :=
   with_closure a ρ κ (VClosure (Lambda e ρ')) :=
-    MkΣ a ρ (Fn (λ v, inl (MkΣ e (Val v ρ') κ))).
+    MkΣ a ρ (Fn (λ v, MkΣ e (Val v ρ') κ)).
 
-Equations step {τ : Ty} (s : Σ τ) : Σ τ + Value τ :=
+(*
+Equations eval
+          {τ : Ty}
+          {Γ : Exp.Env}
+          (e : Exp Γ τ)
+          (ρ : Env Γ) : Value τ :=
+  (* Constants *)
+  eval (Constant x) _ := VConst x;
+
+  eval EUnit  _ := VUnit;
+  eval ETrue  _ := VTrue;
+  eval EFalse _ := VFalse;
+
+  eval (If b t e) ρ with eval b ρ := {
+    | VTrue  => eval t ρ
+    | VFalse => eval e ρ
+  };
+
+  eval (Pair x y) ρ := VPair (eval x ρ) (eval y ρ);
+  eval (Fst p) ρ    := VFst (eval p ρ);
+  eval (Snd p) ρ    := VSnd (eval p ρ);
+
+  (* A sequence just evaluates the second, for now *)
+  eval (Seq _ e2) ρ := eval e2 ρ;
+
+  (* Let is a simple desugaring *)
+  eval (Let x body) ρ := eval body (Val (eval x ρ) ρ);
+
+  (* A variable might lookup a lambda, in which case continue evaluating down
+     that vein; otherwise, if no continuation, this is as far as we can go. *)
+  eval (VAR v) ρ := get ρ v;
+
+  (* If a lambda is passed, call it with the continuation *)
+  eval (LAM e) ρ := VClosure (Lambda e ρ);
+
+  (* Application evaluates the lambda and then the argument *)
+  eval (APP e1 e2) ρ with eval e1 ρ := {
+    | VClosure (Lambda e ρ') => eval e (Val (eval e2 ρ) ρ')
+  }.
+*)
+
+Equations step {τ : Ty} (s : Σ τ) : Σ τ :=
+  step (MkV v) := MkV v;
+
   (* Constants *)
   step (MkΣ (Constant x) _ (Fn f)) := f (VConst x);
 
   step (MkΣ EUnit  _ (Fn f)) := f VUnit;
   step (MkΣ ETrue  _ (Fn f)) := f VTrue;
   step (MkΣ EFalse _ (Fn f)) := f VFalse;
+
   step (MkΣ (If b t e) ρ κ) :=
-    inl (MkΣ b ρ (Fn (λ v, inl (MkΣ (IfBody t e v) ρ κ))));
+    MkΣ b ρ (Fn (λ v, MkΣ (IfBody v t e) ρ κ));
 
   step (MkΣ (Pair x y) ρ (Fn f)) :=
-    inl (MkΣ x ρ (Fn (λ v1, inl (MkΣ y ρ (Fn (λ v2, f (VPair v1 v2)))))));
+    MkΣ x ρ (Fn (λ v1, MkΣ y ρ (Fn (λ v2, f (VPair v1 v2)))));
   step (MkΣ (Fst p) ρ (Fn f)) :=
-    inl (MkΣ p ρ (Fn (f ∘ VFst)));
+    MkΣ p ρ (Fn (f ∘ VFst));
   step (MkΣ (Snd p) ρ (Fn f)) :=
-    inl (MkΣ p ρ (Fn (f ∘ VSnd)));
+    MkΣ p ρ (Fn (f ∘ VSnd));
 
   (* A sequence just evaluates the second, for now *)
   step (MkΣ (Seq e1 e2) ρ κ) :=
-    inl (MkΣ e2 ρ κ);
+    MkΣ e2 ρ κ;
 
   (* Let is a simple desugaring *)
   step (MkΣ (Let x body) ρ κ) :=
-    inl (MkΣ (APP (LAM body) x) ρ κ);
+    MkΣ (APP (LAM body) x) ρ κ;
 
   (* A variable might lookup a lambda, in which case continue evaluating down
      that vein; otherwise, if no continuation, this is as far as we can go. *)
   step (MkΣ (VAR v) ρ κ) with get ρ v := {
-    | VClosure (Lambda e ρ') => inl (MkΣ (LAM e) ρ' κ)
+    | VClosure (Lambda e ρ') => MkΣ (LAM e) ρ' κ
     | x with κ := {
         | Fn f => f x
       }
@@ -137,74 +180,57 @@ Equations step {τ : Ty} (s : Σ τ) : Σ τ + Value τ :=
 
   (* Application evaluates the lambda and then the argument *)
   step (MkΣ (APP e1 e2) ρ κ) :=
-    inl (MkΣ e1 ρ (Fn (inl ∘ with_closure e2 ρ κ))).
+    MkΣ e1 ρ (Fn (with_closure e2 ρ κ)).
 
-Equations loop (gas : nat) {τ : Ty} (s : Σ τ) : Σ τ + Value τ :=
-  loop O s := inl s;
+Equations loop (gas : nat) {τ : Ty} (s : Σ τ) : Σ τ :=
+  loop O s := s;
   loop (S gas') s with step s := {
-    | inl s' => loop gas' s'
-    | inr r  => inr r
+    | MkV v  => MkV v
+    | s' => loop gas' s'
   }.
 
-Definition run (gas : nat) {τ : Ty} {Γ : Exp.Env} (e : Exp Γ τ) (E : Env Γ) :
-  Σ τ + Value τ := loop gas (inject e E).
+Definition run (gas : nat) {τ : Ty} (e : Exp [] τ) : Σ τ := loop gas (inject e).
 
 Example exp_constant :
-  run 10 (Constant (LInteger 123%Z)) Empty = inr (VConst (LInteger 123%Z)).
+  run 10 (Constant (LInteger 123%Z)) = MkV (VConst (LInteger 123%Z)).
 Proof. reflexivity. Qed.
 
 Example exp_pair :
   run 20 (Pair (Constant (LInteger 123%Z))
-               (Constant (LInteger 456%Z))) Empty =
-    inr (VPair (VConst (LInteger 123%Z))
+               (Constant (LInteger 456%Z))) =
+    MkV (VPair (VConst (LInteger 123%Z))
                (VConst (LInteger 456%Z))).
 Proof. reflexivity. Qed.
 
 Example exp_let :
-  run 10 (Let (Constant (LInteger 123%Z)) (VAR ZV)) Empty =
-    inr (VConst (LInteger 123%Z)).
-Proof. reflexivity. Qed.
-
-Example exp_var :
-  run 10 (VAR ZV) (Val (VConst (LInteger 123%Z)) Empty) =
-    inr (VConst (LInteger 123%Z)).
+  run 10 (Let (Constant (LInteger 123%Z)) (VAR ZV)) =
+    MkV (VConst (LInteger 123%Z)).
 Proof. reflexivity. Qed.
 
 Example exp_lam τ :
-  run 10 (LAM (cod:=τ) (VAR ZV)) Empty =
-    inr (VClosure (Lambda (VAR ZV) Empty)).
+  run 10 (LAM (cod:=τ) (VAR ZV)) =
+    MkV (VClosure (Lambda (VAR ZV) Empty)).
 Proof. reflexivity. Qed.
 
 Example exp_app :
-  run 10 (APP (LAM (VAR ZV)) (Constant (LInteger 123%Z))) Empty =
-    inr (VConst (LInteger 123%Z)).
+  run 10 (APP (LAM (VAR ZV)) (Constant (LInteger 123%Z))) =
+    MkV (VConst (LInteger 123%Z)).
 Proof. reflexivity. Qed.
 
-Theorem cek_sound τ (e : Exp [] τ) v v' :
-  e --->* v → represents [] v v' →
-  ∃ gas, loop gas (inject e Empty) = inr v'.
+Ltac ceksimp :=
+  repeat (simp loop;
+          simp step;
+          simp IfBody;
+          simp VFst;
+          simp VSnd;
+          simpl).
+
+Ltac is_step := ceksimp; firstorder eauto.
+
+Theorem cek_sound τ (e e' : Exp [] τ) :
+  e --->* e' → ValueP e' →      (* evaluation halts at e' *)
+  ∃ v, represents e' v ∧ ∃ gas, loop gas (inject e) = MkV v.
 Proof.
-  intros.
-  unfold inject.
-  induction H.
-  - dependent induction x;
-    exists 10%nat;
-    simp loop; simp step; simpl;
-    inv H0; auto.
-    + admit.
-    + now dependent elimination ρ.
-  - destruct IHmulti; auto.
-    induction H;
-    try solve [ exists (S x0);
-                simp loop; simp step; simpl;
-                rewrite <- H1; clear H1 ].
-    + exists (S (S x0)).
-      simp loop; simp step; simpl.
-      now simp loop; simp step; simpl.
-    + exists (S (S x0)).
-      simp loop; simp step; simpl.
-      now simp loop; simp step; simpl.
-    + exists x0.
 Abort.
 
 End CEK.
